WIP

theories/Dot/lr/unary_lr.v
@@ -1,18 +1,24 @@
 From iris.proofmode Require Import tactics.
 From D Require Export iris_prelude.
-From D Require Import ty_interp_subst_lemmas.
+From D Require Import ty_interp_subst_lemmas lty.
 From D.Dot Require Export dlang_inst path_wp.
+
+Notation "'λI' x .. y , t" := (fun x => .. (fun y => t%I) ..)
+  (at level 200, x binder, y binder, right associativity, only parsing,
+  format "'[  ' '[  ' 'λI'  x  ..  y ']' ,  '/' t ']'") : function_scope.
 
 (** Override notation from [dlang] to specify scope. *)
 Notation "⟦ T ⟧" := (ty_interp T%ty).
 
 Include TyInterpLemmas VlSorts dlang_inst.
+Include LtyJudgements VlSorts dlang_inst.
+(* Import SemTypes. *)
 
 (** Deduce types from variable names, like on paper, for readability and to help
     type inference for some overloaded operations (e.g. substitution). *)
 Implicit Types
          (L T U : ty) (v w : vl) (e : tm) (d : dm) (ds : dms) (p : path)
-         (Γ : ctx) (vs : vls) (ρ : var → vl).
+         (vs : vls) (ρ : var → vl).
 
 (** The logical relation core is the [interp], interprets *open* types into
     predicates over *closed* values. Hence, [interp T ρ v] uses its argument [ρ]
@@ -50,82 +56,84 @@ Definition prim_evals_to (B : base_ty) (v : vl) : prim_sem B → Prop :=
 
 Definition pure_interp_prim B v := ∃ l : prim_sem B, prim_evals_to B v l.
 
-Section logrel.
-  Context `{!dlangG Σ}.
+Record dlty Σ := Dlty {
+  dlty_label : label;
+  dlty_car : env -d> dm -d> iPropO Σ;
+  dlty_persistent ρ d :> Persistent (dlty_car ρ d);
+}.
+Global Arguments Dlty {_} _%I _ {_}.
+Global Arguments dlty_car {_} !_ _ _ /.
+Global Arguments dlty_label {_} _ /.
+Global Existing Instance dlty_persistent.
 
-  Notation D := (vl -d> iPropO Σ).
-  Implicit Types (interp φ : envD Σ) (ψ : D).
+Definition lift_dlty `{!dlangG Σ} (φ : dlty Σ) l : envPred dm Σ :=
+  λI ρ d, ⌜ dlty_label φ = l ⌝ ∧ dlty_car φ ρ d.
 
-  Definition def_interp_vmem interp : envPred dm Σ :=
-    λ ρ d, (∃ pmem, ⌜d = dpt pmem⌝ ∧ path_wp pmem (interp ρ))%I.
-  Global Arguments def_interp_vmem /.
+Definition dm_to_type `{!dlangG Σ} d i (ψ : hoD Σ i) : iProp Σ :=
+  (∃ s σ, ⌜ d = dtysem σ s ⌝ ∧ s ↗n[ σ , i ] ψ)%I.
+Notation "d ↗n[ i  ] ψ" := (dm_to_type d i ψ) (at level 20).
 
-  Definition dm_to_type d ψ : iProp Σ :=
-    ∃ s σ, ⌜ d = dtysem σ s ⌝ ∧ s ↗[ σ ] ψ.
-  Notation "d ↗ ψ" := (dm_to_type d ψ) (at level 20).
-  Global Instance dm_to_type_persistent d ψ: Persistent (d ↗ ψ) := _.
+Section dm_to_type.
+  Context `{HdotG: dlangG Σ}.
 
-  Lemma dm_to_type_agree d ψ1 ψ2 v : d ↗ ψ1 -∗ d ↗ ψ2 -∗ ▷ (ψ1 v ≡ ψ2 v).
+  Global Instance dm_to_type_persistent d i ψ: Persistent (d ↗n[ i ] ψ) := _.
+
+  Lemma dm_to_type_agree d i ψ1 ψ2 args v : d ↗n[ i ] ψ1 -∗ d ↗n[ i ] ψ2 -∗ ▷ (ψ1 args v ≡ ψ2 args v).
   Proof.
     iDestruct 1 as (s σ ?) "#Hs1".
     iDestruct 1 as (s' σ' ?) "#Hs2".
-    simplify_eq. by iApply (stamp_σ_to_type_agree vnil with "Hs1 Hs2").
+    simplify_eq. by iApply (stamp_σ_to_type_agree args with "Hs1 Hs2").
   Qed.
 
-  Lemma dm_to_type_intro d s σ φ :
-    d = dtysem σ s → s ↝ φ -∗ d ↗ φ (∞ σ).
+  Lemma dm_to_type_intro d i s σ φ :
+    d = dtysem σ s → s ↝n[ i ] φ -∗ d ↗n[ i ] hoEnvD_inst σ φ.
   Proof.
     iIntros. iExists s, σ. iFrame "%".
     by iApply stamp_σ_to_type_intro.
   Qed.
 
-  Definition dm_to_type_eq d ψ : dm_to_type d ψ =
-    (∃ s σ, ⌜ d = dtysem σ s ⌝ ∧ s ↗[ σ ] ψ)%I := eq_refl.
+  Definition dm_to_type_eq d i ψ : dm_to_type d i ψ =
+    (∃ s σ, ⌜ d = dtysem σ s ⌝ ∧ s ↗n[ σ , i ] ψ)%I := eq_refl.
+
   Global Opaque dm_to_type.
+End dm_to_type.
 
-  Definition def_interp_tmem interp1 interp2 : envPred dm Σ :=
-    λ ρ d,
-    (∃ ψ, (d ↗ ψ) ∧
-       □ ((∀ v, ▷ interp1 ρ v → ▷ □ ψ v) ∧
-          (∀ v, ▷ □ ψ v → ▷ interp2 ρ v)))%I.
-  Global Arguments def_interp_tmem /.
+Section SemTypes.
+  Context `{HdotG: dlangG Σ}.
 
-  Definition lift_dinterp_vl l (dinterp: envPred dm Σ): envD Σ :=
-    λ ρ v, (∃ d, ⌜v @ l ↘ d⌝ ∧ dinterp ρ d)%I.
-  Global Arguments lift_dinterp_vl /.
+  Implicit Types (τ : olty Σ 0).
+   (* (ψ : vl -d> iPropO Σ) (φ : envD Σ)  *)
 
-  Definition interp_vmem l interp : envD Σ :=
-    lift_dinterp_vl l (def_interp_vmem interp).
-  Global Arguments interp_vmem /.
+  Program Definition lift_dinterp_vl (T : dlty Σ): olty Σ 0 :=
+    olty0 (λI ρ v, (∃ d, ⌜v @ dlty_label T ↘ d⌝ ∧ dlty_car T ρ d)).
 
-  Definition interp_tmem l interp1 interp2 : envD Σ :=
-    lift_dinterp_vl l (def_interp_tmem interp1 interp2).
-  Global Arguments interp_tmem /.
+  (* Rewrite using (higher) semantic kinds! *)
+  Definition oDTMem l τ1 τ2 : dlty Σ := Dlty l
+    (λI ρ d,
+    ∃ ψ, (d ↗n[ 0 ] ψ) ∧
+       □ ((∀ v, ▷ τ1 vnil ρ v → ▷ □ ψ vnil v) ∧
+          (∀ v, ▷ □ ψ vnil v → ▷ τ2 vnil ρ v))).
 
-  Definition interp_expr interp : envPred tm Σ :=
-    λ ρ t, (□ WP t {{ interp ρ }})%I.
-  Global Arguments interp_expr /.
+  Definition oTTMem l τ1 τ2 :=
+    lift_dinterp_vl (oDTMem l τ1 τ2).
 
-  Definition interp_and interp1 interp2 : envD Σ :=
-    λ ρ v, (interp1 ρ v ∧ interp2 ρ v)%I.
-  Global Arguments interp_and /.
+  Definition oDVMem l τ : dlty Σ := Dlty l
+    (λI ρ d, ∃ pmem, ⌜d = dpt pmem⌝ ∧ path_wp pmem (oClose τ ρ)).
 
-  Definition interp_or interp1 interp2 : envD Σ :=
-    λ ρ v, (interp1 ρ v ∨ interp2 ρ v)%I.
-  Global Arguments interp_or /.
+  Definition oTVMem l τ :=
+    lift_dinterp_vl (oDVMem l τ).
 
-  Definition interp_later interp : envD Σ :=
-    λ ρ v, (▷ interp ρ v)%I.
-  Global Arguments interp_later /.
+  Definition oTSel p (l : label) :=
+    olty0 (λI ρ v, path_wp p.|[ρ]
+      (λ vp, ∃ ψ d, ⌜vp @ l ↘ d⌝ ∧ d ↗n[ 0 ] ψ ∧ ▷ □ ψ vnil v)).
 
-  Definition interp_prim b : envD Σ := λ ρ v, ⌜pure_interp_prim b v⌝%I.
-  Global Arguments interp_prim /.
+  Lemma oTSel_pv w (l : label) args ρ v :
+    oTSel (pv w) l args ρ v ⊣⊢
+      ∃ ψ d, ⌜w.[ρ] @ l ↘ d⌝ ∧ d ↗n[ 0 ] ψ ∧ ▷ □ ψ vnil v.
+  Proof. by rewrite /= path_wp_pv. Qed.
 
-  Definition interp_top : envD Σ := λ ρ v, True%I.
-  Global Arguments interp_top /.
-
-  Definition interp_bot : envD Σ := λ ρ v, False%I.
-  Global Arguments interp_bot /.
+  Definition oPSing p : olty Σ 0 :=
+    olty0 (λI ρ v, ⌜alias_paths p.|[ρ] (pv v)⌝).
 
   (* Paolo: This definition is contractive (similarly to what's useful for
      equi-recursive types).
@@ -138,188 +146,147 @@ Section logrel.
      typechecking this example needs to establish x.T <: TNat having in context
      only x: {T <: TNat; U <: x.T -> TNat}.
    *)
-  Definition interp_forall interp1 interp2 : envD Σ :=
-    λ ρ v,
+  Definition oForall τ1 τ2 := olty0
+    (λI ρ v,
     (∃ t, ⌜ v = vabs t ⌝ ∧
-     □ ∀ w, ▷ interp1 ρ w → ▷ interp_expr interp2 (w .: ρ) t.|[w/])%I.
-  Global Arguments interp_forall /.
+     □ ∀ w, ▷ τ1 vnil ρ w → ▷ interp_expr τ2 (w .: ρ) t.|[w/])).
 
-  Definition interp_mu interp : envD Σ :=
-    λ ρ v, interp (v .: ρ) v.
-  Global Arguments interp_mu /.
+  Definition oPrim b : olty Σ 0 := olty0 (λI ρ v, ⌜pure_interp_prim b v⌝).
 
-  Definition interp_sel p (l: label) : envD Σ :=
-    λ ρ v, (path_wp p.|[ρ]
-      (λ vp, ∃ ψ d, ⌜vp @ l ↘ d⌝ ∧ d ↗ ψ ∧ ▷ □ ψ v))%I.
-  Global Arguments interp_sel /.
+  Class PersTyInterp (ty : Type) Σ :=
+    pers_ty_interp : ty → olty Σ 0.
+  Notation "p⟦ T ⟧" := (pers_ty_interp T%ty).
+  Global Arguments pers_ty_interp {_ _ _} !_ /.
 
-  Definition interp_sing p : envD Σ :=
-    λ ρ v, ⌜alias_paths p.|[ρ] (pv v)⌝%I.
-  Global Arguments interp_sing /.
-
-  Global Instance interp : TyInterp ty Σ := fix interp (T : ty) : envD Σ :=
-    let _ := interp : TyInterp ty Σ in
+  Global Instance pinterp : PersTyInterp ty Σ :=
+    fix pinterp (T : ty) : olty Σ 0 :=
+    let _ := pinterp : PersTyInterp ty Σ in
     match T with
-    | TTMem l L U => interp_tmem l ⟦ L ⟧ ⟦ U ⟧
-    | TVMem l T' => interp_vmem l ⟦ T' ⟧
-    | TAnd T1 T2 => interp_and ⟦ T1 ⟧ ⟦ T2 ⟧
-    | TOr T1 T2 => interp_or ⟦ T1 ⟧ ⟦ T2 ⟧
-    | TLater T => interp_later ⟦ T ⟧
-    | TPrim b => interp_prim b
-    | TTop => interp_top
-    | TBot => interp_bot
-    | TAll T1 T2 => interp_forall ⟦ T1 ⟧ ⟦ T2 ⟧
-    | TMu T => interp_mu ⟦ T ⟧
-    | TSel p l => interp_sel p l
-    | TSing p => interp_sing p
-    end%I.
+    | TTMem l L U => oTTMem l p⟦ L ⟧ p⟦ U ⟧
+    | TVMem l T' => oTVMem l p⟦ T' ⟧
+    | TAnd T1 T2 => oAnd p⟦ T1 ⟧ p⟦ T2 ⟧
+    | TOr T1 T2 => oOr p⟦ T1 ⟧ p⟦ T2 ⟧
+    | TLater T => oLater p⟦ T ⟧
+    | TPrim b => oPrim b
+    | TTop => oTop
+    | TBot => oBot
+    | TAll T1 T2 => oForall p⟦ T1 ⟧ p⟦ T2 ⟧
+    | TMu T => oMu p⟦ T ⟧
+    | TSel p l => oTSel p l
+    | TSing p => oPSing p
+    end.
+  (* Wrap this into ty_interp to reuse lemmas. *)
+  Global Instance pers_to_ty_interp : TyInterp ty Σ := flip pers_ty_interp vnil.
+  Global Arguments pers_to_ty_interp _ /.
+  Global Arguments ty_interp {_ _ _} _ /.
 
   Global Instance interp_lemmas: TyInterpLemmas ty Σ.
   Proof.
-    split; induction T => sb1 sb2 w /=;
-      properness; rewrite /= ?scons_up_swap ?hsubst_comp; trivial; by f_equiv => ?.
+    split => /=; induction T => sb1 sb2 w /=;
+      properness; rewrite ?scons_up_swap ?hsubst_comp; trivial; by f_equiv => ?.
   Qed.
 
-  Notation "⟦ T ⟧ₑ" := (interp_expr ⟦ T ⟧).
+  Global Instance interp_persistent T ρ v : Persistent (⟦ T ⟧ ρ v) := _.
 
-  Global Instance interp_persistent T ρ v :
-    Persistent (⟦ T ⟧ ρ v).
-  Proof. revert v ρ; induction T => w ρ /=; try apply _. Qed.
-
-  Fixpoint def_interp_base (T : ty) : envPred dm Σ :=
-    λ ρ d,
+  Fixpoint def_interp_base (T : ty) : dlty Σ :=
     match T with
-    | TTMem _ L U => def_interp_tmem ⟦ L ⟧ ⟦ U ⟧ ρ d
-    | TVMem _ T' => def_interp_vmem ⟦ T' ⟧ ρ d
-    | _ => False
-    end%I.
+    | TTMem l L U => oDTMem l p⟦ L ⟧ p⟦ U ⟧
+    | TVMem l T' => oDVMem l p⟦ T' ⟧
+    | _ => Dlty "" (λI _ _, False)
+    end.
 
-  Definition def_interp (T : ty) l : envPred dm Σ :=
-    λ ρ d,
-    (⌜ label_of_ty T = Some l ⌝ ∧ def_interp_base T ρ d)%I.
-
-  Global Instance def_interp_base_persistent T ρ d :
-    Persistent (def_interp_base T ρ d).
+  Global Instance def_interp_persistent T ρ d :
+    Persistent (dlty_car (def_interp_base T) ρ d).
   Proof. destruct T; try apply _. Qed.
 
-  Global Instance def_interp_persistent T l ρ d :
-    Persistent (def_interp T l ρ d) := _.
+  Implicit Types (l : label).
+
+  Definition def_interp T l := lift_dlty (def_interp_base T) l.
 
   Definition defs_interp_and (interp1 interp2 : envPred dms Σ) : envPred dms Σ :=
-    λ ρ ds, (interp1 ρ ds ∧ interp2 ρ ds)%I.
+    λI ρ ds, interp1 ρ ds ∧ interp2 ρ ds.
 
-  Definition lift_dinterp_dms T : envPred dms Σ := λ ρ ds, (∃ l d,
-    ⌜ dms_lookup l ds = Some d ⌝
-    ∧ def_interp T l ρ d)%I.
+  Definition lift_dinterp_dms T : envPred dms Σ := λI ρ ds,
+    ∃ l d, ⌜ dms_lookup l ds = Some d ⌝ ∧ def_interp T l ρ d.
 
   Fixpoint defs_interp T : envPred dms Σ :=
     match T with
     | TAnd T1 T2 => defs_interp_and (defs_interp T1) (defs_interp T2)
-    | TTop => λ ρ ds, True
+    | TTop => λI ρ ds, True
     | _ => lift_dinterp_dms T
-    end%I.
+    end.
 
   Global Instance defs_interp_persistent T ρ ds : Persistent (defs_interp T ρ ds).
   Proof. induction T; try apply _. Qed.
 
-  Fixpoint interp_env (Γ : ctx) (ρ : var → vl) : iProp Σ :=
+  (* Fixpoint interp_env (Γ : ctx) (ρ : var → vl) : iProp Σ :=
     match Γ with
     | T :: Γ' => interp_env Γ' (stail ρ) ∧ ⟦ T ⟧ ρ (shead ρ)
     | nil => True
-    end%I.
+    end%I. *)
+End SemTypes.
 
-  Notation "⟦ Γ ⟧*" := (interp_env Γ).
+Notation "d ↗ ψ" := (dm_to_type 0 d ψ) (at level 20).
+Notation "p⟦ T ⟧" := (pers_ty_interp T%ty).
+Notation "p⟦ Γ ⟧*" := (pers_ty_interp <$> Γ).
+Notation "p⟦ T ⟧ₑ" := (interp_expr ⟦ T ⟧).
+(* Notation "⟦ T ⟧ₑ" := (interp_expr p⟦ T ⟧). *)
+(* Definition interp_env (Γ : ctx) : env -d> iPropO Σ := env_oltyped (pers_ty_interp <$> Γ).
+Global Arguments interp_env !_ _ /.
+Notation "⟦ Γ ⟧*" := (interp_env Γ). *)
+(* Notation "⟦ Γ ⟧*" := (env_oltyped (pers_ty_interp <$> Γ)). *)
+Notation "⟦ Γ ⟧*" := s⟦ p⟦ Γ ⟧* ⟧*.
 
-  Global Instance interp_env_persistent Γ ρ :
-    Persistent (⟦ Γ ⟧* ρ).
-  Proof. elim: Γ ρ => [|τ Γ IHΓ] ρ /=; apply _. Qed.
+(* Definition idtp `{!dlangG Σ} Γ l (φ : dlty Σ) d : iProp Σ :=
+  (⌜ dlty_label φ = l ⌝ ∧
+    □∀ ρ, ⟦Γ⟧* ρ → dlty_car φ ρ d.|[ρ])%I. *)
+Definition idtp `{!dlangG Σ} Γ l (φ : dlty Σ) d : iProp Σ :=
+  □∀ ρ, ⌜path_includes (pv (ids 0)) ρ [(l, d)] ⌝ → s⟦Γ⟧* ρ → lift_dlty φ l ρ d.|[ρ].
+Global Arguments idtp /.
+Notation "Γ s⊨ { l := d  } : T" := (idtp Γ l T d) (at level 74, d, l, T at next level).
 
-  (** Definitions for semantic (definition) (sub)typing *)
-  Definition idtp Γ T l d : iProp Σ :=
-    □∀ ρ, ⌜path_includes (pv (ids 0)) ρ [(l, d)] ⌝ → ⟦Γ⟧* ρ → def_interp T l ρ d.|[ρ].
-  Global Arguments idtp /.
+Definition idstp `{!dlangG Σ} Γ T ds : iProp Σ :=
+  ⌜wf_ds ds⌝ ∧ □∀ ρ, ⌜path_includes (pv (ids 0)) ρ ds ⌝ → s⟦Γ⟧* ρ → defs_interp T ρ ds.|[ρ].
+Global Arguments idstp /.
+(** Multi-definition typing *)
+Notation "Γ s⊨ds ds : T" := (idstp Γ T ds) (at level 74, ds, T at next level).
 
-  Definition idstp Γ T ds : iProp Σ :=
-    ⌜wf_ds ds⌝ ∧ □∀ ρ, ⌜path_includes (pv (ids 0)) ρ ds ⌝ → ⟦Γ⟧* ρ → defs_interp T ρ ds.|[ρ].
-  Global Arguments idstp /.
-
-  Definition ietp Γ T e : iProp Σ :=
-    □∀ ρ, ⟦Γ⟧* ρ → ⟦T⟧ₑ ρ (e.|[ρ]).
-  Global Arguments ietp /.
-
-  (** Indexed Subtyping. Defined on closed values. We must require closedness
-      explicitly, since closedness now does not follow from being well-typed later. *)
-  (** How do we represent subtyping in a later world? We have two distinct
-      choices, because in Iris ▷(P ⇒ Q) ⊢ ▷ P ⇒ ▷ Q but not viceversa
-      (unlike with raw step-indexing).
-      In turn, that's because to show ▷ P ⇒ ▷ Q we can assume resources are
-      valid one step earlier, unlike for ▷(P ⇒ Q).
-
-      It seems easier, in subtyping judgment, to use the weaker choice: that is,
-      just delay individual types via (Γ ⊨ TLater T <: TLater U), that is
-
-      (□∀ v ρ, ⟦Γ⟧* ρ → ▷ ⟦T1⟧ ρ v → ▷ ⟦T2⟧ ρ v),
-
-      instead of instead of introducing some notation to write
-
-      (□∀ v ρ, ⟦Γ⟧* ρ → ▷ (⟦T1⟧ ρ v → ⟦T2⟧ ρ v)).
-
-      And that forces using the same implication in the logical relation
-      (unlike I did originally). *)
-  Definition step_indexed_ivstp Γ T1 T2 i j: iProp Σ :=
-    □∀ ρ v, ⟦Γ⟧* ρ → ▷^i ⟦T1⟧ ρ v → ▷^j ⟦T2⟧ ρ v.
-
-  Global Arguments step_indexed_ivstp /.
-
-  Definition iptp Γ T p i: iProp Σ :=
-    □∀ ρ, ⟦Γ⟧* ρ →
-     ▷^i path_wp p.|[ρ] (λ v, ⟦T⟧ ρ v).
-  Global Arguments iptp /.
-
-  Local Notation IntoPersistent' P := (IntoPersistent false P P).
-
-  (* Avoid auto-dropping box (and unfolding) when introducing judgments persistently. *)
-  Global Instance idtp_persistent Γ T l d: IntoPersistent' (idtp Γ T l d) | 0 := _.
-  Global Instance idstp_persistent Γ T ds: IntoPersistent' (idstp Γ T ds) | 0 := _.
-  Global Instance ietp_persistent Γ T e : IntoPersistent' (ietp Γ T e) | 0 := _.
-  Global Instance step_indexed_ivstp_persistent Γ T1 T2 i j : IntoPersistent' (step_indexed_ivstp Γ T1 T2 i j) | 0 := _.
-  Global Instance iptp_persistent Γ T p i : IntoPersistent' (iptp Γ T p i) | 0 := _.
-End logrel.
-
-Notation "d ↗ ψ" := (dm_to_type d ψ) (at level 20).
-Notation "⟦ Γ ⟧*" := (interp_env Γ).
-Notation "⟦ T ⟧ₑ" := (interp_expr ⟦ T ⟧).
+Definition iptp `{!dlangG Σ} Γ (τ : olty Σ 0) p i: iProp Σ :=
+  □∀ ρ, ⟦Γ⟧* ρ -∗
+    ▷^i path_wp (p.|[ρ]) (λ v, oClose τ ρ v).
+Global Arguments iptp /.
+Notation "Γ s⊨p p : τ , i" := (iptp Γ τ p i) (at level 74, p, τ, i at next level).
 
 (** Single-definition typing *)
-Notation "Γ ⊨ {  l := d  } : T" := (idtp Γ T l d) (at level 74, d, l, T at next level).
+Notation "Γ ⊨ {  l := d  } : T" := (idtp p⟦Γ⟧* p⟦T⟧ l d) (at level 74, d, l, T at next level).
 (** Multi-definition typing *)
-Notation "Γ ⊨ds ds : T" := (idstp Γ T ds) (at level 74, ds, T at next level).
+Notation "Γ ⊨ds ds : T" := (idstp p⟦Γ⟧* p⟦T⟧ ds) (at level 74, ds, T at next level).
 (** Expression typing *)
-Notation "Γ ⊨ e : T" := (ietp Γ T e) (at level 74, e, T at next level).
+Notation "Γ ⊨ e : T" := (ietp p⟦Γ⟧* p⟦T⟧ e) (at level 74, e, T at next level).
+Notation "Γ ⊨p p : T , i" := (iptp p⟦Γ⟧* p⟦T⟧ p i) (at level 74, p, T, i at next level).
 
-Notation "Γ ⊨p p : T , i" := (iptp Γ T p i) (at level 74, p, T, i at next level).
-
-Notation "Γ ⊨ T1 , i <: T2 , j " := (step_indexed_ivstp Γ T1 T2 i j) (at level 74, T1, T2, i, j at next level).
+Notation "Γ ⊨ T1 , i <: T2 , j " := (step_indexed_ivstp p⟦Γ⟧* p⟦T1⟧ p⟦T2⟧ i j) (at level 74, T1, T2, i, j at next level).
 
 Import stamp_transfer.
 (** Single-definition typing *)
-Notation "Γ ⊨[ gφ  ] { l := d  } : T" := (wellMappedφ gφ → idtp Γ T l d)%I (at level 74, d, l, T at next level).
+Notation "Γ ⊨[ gφ  ] { l := d  } : T" := (wellMappedφ gφ → Γ ⊨ {  l := d  } : T)%I (at level 74, d, l, T at next level).
 (** Multi-definition typing *)
-Notation "Γ ⊨ds[ gφ  ] ds : T" := (wellMappedφ gφ → idstp Γ T ds)%I (at level 74, ds, T at next level).
+Notation "Γ ⊨ds[ gφ  ] ds : T" := (wellMappedφ gφ → Γ ⊨ds ds : T)%I (at level 74, ds, T at next level).
 (** Expression typing *)
-Notation "Γ ⊨[ gφ  ] e : T" := (wellMappedφ gφ → ietp Γ T e)%I (at level 74, e, T at next level).
-Notation "Γ ⊨p[ gφ  ] p : T , i" := (wellMappedφ gφ → iptp Γ T p i)%I (at level 74, p, T, i at next level).
-Notation "Γ ⊨[ gφ  ] T1 , i <: T2 , j" := (wellMappedφ gφ → step_indexed_ivstp Γ T1 T2 i j)%I (at level 74, T1, T2, i, j at next level).
+Notation "Γ ⊨[ gφ  ] e : T" := (wellMappedφ gφ → Γ ⊨ e : T)%I (at level 74, e, T at next level).
+Notation "Γ ⊨p[ gφ  ] p : T , i" := (wellMappedφ gφ → Γ ⊨p p : T , i)%I (at level 74, p, T, i at next level).
+Notation "Γ ⊨[ gφ  ] T1 , i <: T2 , j" := (wellMappedφ gφ → Γ ⊨ T1 , i <: T2 , j)%I (at level 74, T1, T2, i, j at next level).
 
 Section logrel_lemmas.
   Context `{!dlangG Σ}.
 
-  Lemma iterate_TLater_later0 i T:
-    ⟦ iterate TLater i T ⟧ ≡ (λ ρ v, ▷^i ⟦ T ⟧ ρ v)%I.
-  Proof. move => ρ v. elim: i => [|i IHi] //. rewrite iterate_S /= IHi //. Qed.
-  Lemma iterate_TLater_later i T ρ v:
+  Lemma iterate_TLater_later0 i T ρ v:
+    oClose (p⟦ iterate TLater i T ⟧) ρ v ≡ oClose (olty0 (λI ρ v, ▷^i p⟦ T ⟧ vnil ρ v)) ρ v.
+  Proof. elim: i => [|i IHi] //. rewrite iterate_S /= IHi //. Qed.
+
+  (* Lemma iterate_TLater_later i T ρ v:
     ⟦ iterate TLater i T ⟧ ρ v ≡ (▷^i ⟦ T ⟧ ρ v)%I.
-  Proof. exact: iterate_TLater_later0. Qed.
+  Proof. exact: iterate_TLater_later0. Qed. *)
 
   Lemma def_interp_tvmem_eq l T p ρ:
     def_interp (TVMem l T) l ρ (dpt p) ⊣⊢
@@ -329,7 +296,7 @@ Section logrel_lemmas.
     iIntros "H"; iSplit; first done; iExists p. by auto.
   Qed.
 
-  Lemma interp_env_lookup Γ ρ T x:
+  Lemma interp_env_lookup' Γ ρ T x:
     Γ !! x = Some T →
     ⟦ Γ ⟧* ρ -∗ ⟦ (shiftN x T) ⟧ ρ (ρ x).
   Proof.
@@ -341,30 +308,43 @@ Section logrel_lemmas.
       iApply (IHΓ (stail ρ) x Hx with "Hg").
   Qed.
 
-  Context {Γ}.
-  Lemma Sub_Refl T i : Γ ⊨ T, i <: T, i.
+  Lemma sSub_Refl Γ (T : olty Σ 0) i : Γ s⊨ T, i <: T, i.
   Proof. by iIntros "!> **". Qed.
+
+  Lemma sSub_Trans Γ (T1 T2 T3 : olty Σ 0) i1 i2 i3 :
+    Γ s⊨ T1, i1 <: T2, i2 -∗
+    Γ s⊨ T2, i2 <: T3, i3 -∗
+    Γ s⊨ T1, i1 <: T3, i3.
+  Proof.
+    iIntros "#Hsub1 #Hsub2 !> * #Hg #HT /=".
+    iApply ("Hsub2" with "[//] (Hsub1 [//] [//])").
+  Qed.
+
+  (* Context {Γ : sCtx Σ}. *)
+  Context {Γ : ctx}.
+  Implicit Type (τ : olty Σ 0).
+
+  Lemma Sub_Refl T i : Γ ⊨ T, i <: T, i.
+  Proof. apply sSub_Refl. Qed.
 
   Lemma Sub_Trans T1 T2 T3 i1 i2 i3 : Γ ⊨ T1, i1 <: T2, i2 -∗
                                       Γ ⊨ T2, i2 <: T3, i3 -∗
                                       Γ ⊨ T1, i1 <: T3, i3.
-  Proof.
-    iIntros "#Hsub1 #Hsub2 !> * #Hg #HT".
-    iApply ("Hsub2" with "[//] (Hsub1 [//] [//])").
-  Qed.
+  Proof. apply sSub_Trans. Qed.
 
   Lemma Sub_Eq T U i j :
     Γ ⊨ T, i <: U, j ⊣⊢
     Γ ⊨ iterate TLater i T, 0 <: iterate TLater j U, 0.
-  Proof. by cbn; setoid_rewrite iterate_TLater_later. Qed.
+  Proof. by cbn; setoid_rewrite iterate_TLater_later0. Qed.
 End logrel_lemmas.
 
 From D Require Import swap_later_impl.
 Import dlang_adequacy adequacy.
 
-Theorem adequacy_dot_sem Σ `{HdlangG: dlangPreG Σ} `{SwapPropI Σ} e Ψ T
-  (Himpl : ∀ (Hdlang: dlangG Σ) v, ⟦ T ⟧ ids v -∗ ⌜Ψ v⌝)
-  (Hlog : ∀ `{dlangG Σ} `(!SwapPropI Σ), allGs ∅ ==∗ [] ⊨ e : T):
+Theorem s_adequacy_dot_sem Σ `{HdlangG: dlangPreG Σ} `{SwapPropI Σ} e Ψ
+  (τ : ∀ `{dlangG Σ}, olty Σ 0)
+  (Himpl : ∀ (Hdlang: dlangG Σ) v, oClose τ ids v -∗ ⌜Ψ v⌝)
+  (Hlog : ∀ `{dlangG Σ} `(!SwapPropI Σ), allGs ∅ ==∗ [] s⊨ e : τ):
   ∀ σ, adequate NotStuck e σ (λ v _, Ψ v).
 Proof.
   eapply (adequacy_dlang _); [apply Himpl | iIntros (??) "Hgs"].
@@ -372,7 +352,19 @@ Proof.
   iEval rewrite -(hsubst_id e). iApply ("Htyp" $! ids with "[//]").
 Qed.
 
+Theorem adequacy_dot_sem Σ `{HdlangG: dlangPreG Σ} `{SwapPropI Σ} e Ψ T
+  (Himpl : ∀ (Hdlang: dlangG Σ) v, ⟦ T ⟧ ids v -∗ ⌜Ψ v⌝)
+  (Hlog : ∀ `{dlangG Σ} `(!SwapPropI Σ), allGs ∅ ==∗ [] ⊨ e : T):
+  ∀ σ, adequate NotStuck e σ (λ v _, Ψ v).
+Proof. exact: (s_adequacy_dot_sem Σ e Ψ (λ _, p⟦T⟧)). Qed.
+
+Corollary s_safety_dot_sem Σ `{HdlangG: dlangPreG Σ} `{SwapPropI Σ} e
+  (τ : ∀ `{dlangG Σ}, olty Σ 0)
+  (Hwp : ∀ `{dlangG Σ} `(!SwapPropI Σ), allGs ∅ ==∗ [] s⊨ e : τ):
+  safe e.
+Proof. apply adequate_safe, (s_adequacy_dot_sem _ e _ τ), Hwp; naive_solver. Qed.
+
 Corollary safety_dot_sem Σ `{HdlangG: dlangPreG Σ} `{SwapPropI Σ} e T
   (Hwp : ∀ `{dlangG Σ} `(!SwapPropI Σ), allGs ∅ ==∗ [] ⊨ e : T):
   safe e.
-Proof. apply adequate_safe, (adequacy_dot_sem _ e _ T), Hwp; naive_solver. Qed.
+Proof. exact: (s_safety_dot_sem Σ e (λ _, p⟦T⟧)). Qed.
